src/Compilers/Named/DeadCodeEliminationInterp.v
@@ -1,0 +1,67 @@
+Require Import Coq.PArith.BinPos.
+Require Import Crypto.Compilers.Syntax.
+Require Import Crypto.Compilers.Named.Context.
+Require Import Crypto.Compilers.Named.PositiveContext.
+Require Import Crypto.Compilers.Named.Syntax.
+Require Import Crypto.Compilers.Named.ContextDefinitions.
+Require Import Crypto.Compilers.Named.RegisterAssignInterp.
+Require Import Crypto.Compilers.Named.DeadCodeElimination.
+Require Import Crypto.Util.Decidable.
+
+Section language.
+  Context {base_type_code : Type}
+          {op : flat_type base_type_code -> flat_type base_type_code -> Type}
+          {interp_base_type : base_type_code -> Type}
+          {interp_op : forall s d, op s d -> interp_flat_type interp_base_type s -> interp_flat_type interp_base_type d}
+          {Name : Type}
+          {InContext : Context Name (fun _ : base_type_code => BinNums.positive)}
+          {InContextOk : ContextOk InContext}
+          {Name_beq : Name -> Name -> bool}
+          {InterpContext : Context Name interp_base_type}
+          {InterpContextOk : ContextOk InterpContext}
+          {base_type_code_beq : base_type_code -> base_type_code -> bool}
+          (base_type_code_bl : forall t1 t2, base_type_code_beq t1 t2 = true -> t1 = t2)
+          (base_type_code_lb : forall t1 t2, t1 = t2 -> base_type_code_beq t1 t2 = true)
+          (Name_bl : forall n1 n2, Name_beq n1 n2 = true -> n1 = n2)
+          (Name_lb : forall n1 n2, n1 = n2 -> Name_beq n1 n2 = true).
+
+  Local Notation EliminateDeadCode := (@EliminateDeadCode base_type_code op Name _ base_type_code_bl InContext).
+  Local Notation PContext var := (@PositiveContext base_type_code var base_type_code_beq base_type_code_bl).
+
+  Local Instance Name_dec : DecidableRel (@eq Name)
+    := dec_rel_of_bool_dec_rel Name_beq Name_bl Name_lb.
+  Local Instance base_type_code_dec : DecidableRel (@eq base_type_code)
+    := dec_rel_of_bool_dec_rel base_type_code_beq base_type_code_bl base_type_code_lb.
+
+  Lemma interp_EliminateDeadCode
+        t e new_names
+        (ctxi_interp : PositiveContext _ _ base_type_code_beq base_type_code_bl)
+        (ctxr_interp : InterpContext)
+        eout v1 v2 x
+    : @EliminateDeadCode t e new_names = Some eout
+      -> interp (interp_op:=interp_op) (ctx:=ctxr_interp) eout x = Some v1
+      -> interp (interp_op:=interp_op) (ctx:=ctxi_interp) e x = Some v2
+      -> v1 = v2.
+  Proof using InContextOk InterpContextOk Name_bl Name_lb base_type_code_lb.
+    eapply @interp_register_reassign;
+      first [ assumption
+            | apply @PositiveContextOk; assumption
+            | apply Peqb_true_eq
+            | apply Pos.eqb_eq
+            | exact _
+            | intros *; rewrite !lookupb_empty by (try apply @PositiveContextOk; assumption);
+              congruence ].
+  Qed.
+
+  Lemma InterpEliminateDeadCode
+        t e new_names
+        eout
+        v1 v2 x
+    : @EliminateDeadCode t e new_names = Some eout
+      -> Interp (Context:=InterpContext) (interp_op:=interp_op) eout x = Some v1
+      -> Interp (Context:=PContext _) (interp_op:=interp_op) e x = Some v2
+      -> v1 = v2.
+  Proof using InContextOk InterpContextOk Name_bl Name_lb base_type_code_lb.
+    apply interp_EliminateDeadCode.
+  Qed.
+End language.
